# Extracting Variable from Expression

## Power

$$
\begin{cases}
\nabla = x^n
\\
x = \sqrt[n]{\nabla}
\end{cases}
$$

$$
\begin{cases}
\nabla = n^x
\\
x = \frac{\ln\nabla}{\ln n} = \log_n\nabla
\end{cases}
$$

## Root

$$
\begin{cases}
\nabla = \sqrt[n]{x}
\\
x = \nabla^n \ \cup\ e^{n\cdot\ln\nabla}
\end{cases}
$$

$$
\begin{cases}
\nabla = \sqrt[x]{n}
\\
x = \frac{1}{\log_n \nabla} = \log_{\nabla} n
\end{cases}
$$

## Logarithm

$$
\begin{cases}
\nabla = \log_n x
\\
x = n^{\nabla}
\end{cases}
$$

$$
\begin{cases}
\nabla = \log_x n
\\
x = \sqrt[\nabla]{n} \ \cup\ e^{\frac{\ln n}{\nabla}}
\end{cases}
$$

## Function

$$
\begin{cases}
\nabla = f(x)
\\
x = f^{-1}(\nabla)
\end{cases}
$$

$$
\begin{cases}
\nabla = \sin/\cos/\tan(x)
\\
x = \arcsin/\arccos/\arctan(\nabla)
\end{cases}
$$

$$
\begin{cases}
\nabla = \sinh/\cosh/\tanh(x)
\\
x = \text{arcsinh/arccosh/arctanh}(\nabla)
\end{cases}
$$

## Others

$$
\begin{cases}
\nabla = (x-n)(x+n)
\\
x = \sqrt{\nabla-n^2}
\end{cases}
$$

$$
\begin{cases}
\nabla = (x+n)^2
\\
x = \sqrt{\nabla}-n
\end{cases}
$$

$$
\begin{cases}
\nabla = (x-n)^2
\\
x = \sqrt{\nabla}+n
\end{cases}
$$

$$
\begin{cases}
\nabla = (n-x)^2
\\
x = n-\sqrt{\nabla}
\end{cases}
$$

$$
\begin{cases}
\nabla = \frac{ax+b}{cx+d}
\\
x = \frac{b-\nabla d}{\nabla c-a}
\end{cases}
$$



